COMPUTING INTEGRALS OF EXAM

For computing $\int_{0}^{\dagger} e^{\tau A} d \tau$ I can simply compute $e^{c}$, where

$$
C=\left[\begin{array}{ll}
A & I \\
0 & 0
\end{array}\right]
$$

To do so we need to compute powers of $C$ :

$$
\begin{aligned}
& C^{2}=\left[\begin{array}{ll}
A & 1 \\
0 & 0
\end{array}\right]\left[\begin{array}{ll}
A & 1 \\
0 & 0
\end{array}\right]=\left[\begin{array}{ll}
A^{2} & A \\
0 & 0
\end{array}\right] \\
& C^{3}=\left[\begin{array}{ll}
A^{2} & A \\
0 & 0
\end{array}\right]\left[\begin{array}{ll}
A & 1 \\
0 & 0
\end{array}\right]=\left[\begin{array}{ll}
A^{3} & A^{2} \\
0 & 0
\end{array}\right] \\
& C^{k}=\left[\begin{array}{ll}
A^{k} & A^{k-1} \\
0 & 0
\end{array}\right] \quad e^{c} \simeq\left(\sum_{k=0} a_{k} C^{k}\right)^{-1}\left(\sum_{k=0} b_{k} C^{k}\right)
\end{aligned}
$$

Good news: we con compute powers of $C$ by only computing powers of $A$ which is half its size, so it should be 8 limes faster.
After computing the powers of $C$ well need $t_{0}$ invert a matrix that hos this structure:

$$
\begin{aligned}
& M=\left[\begin{array}{cc}
M_{1} & M_{2} \\
0 & \alpha I
\end{array}\right] \quad M^{-1}=\left[\begin{array}{ll}
N_{1} & N_{2} \\
N_{3} & N_{4}
\end{array}\right] \quad \alpha=a_{0} \in \mathbb{R} \\
& M M^{-1}=\left[\begin{array}{cc}
M_{1} & M_{2} \\
0 & \alpha I
\end{array}\right]\left[\begin{array}{ll}
N_{1} & N_{2} \\
N_{3} & N_{4}
\end{array}\right]=\left[\begin{array}{cc}
M_{1} N_{1}+M_{2} N_{3} & M_{1} N_{2}+M_{2} N_{4} \\
\alpha N_{3} & \alpha N_{4}
\end{array}\right]
\end{aligned}
$$

So we know that $N_{3}=0, N_{4}=\alpha^{-1} I$ and:

$$
\left\{\begin{array} { l } 
{ M _ { 1 } N _ { 1 } = I } \\
{ M _ { 1 } N _ { 2 } + \alpha ^ { - 1 } M _ { 2 } = 0 }
\end{array} \quad \left\{\begin{array}{l}
N_{1}=M_{1}^{-1} \\
N_{2}=-\alpha^{-1} M_{1}^{-1} M_{2}
\end{array}\right.\right.
$$

We only need to invert $M, t_{0}$ compute the inverse of $M$

Maybe the same trick can be applied to compute

$$
\begin{array}{ll}
x_{\text {in }} t(t)=\int_{0}^{T} x(\tau) d \tau & x_{\text {int }}(t)=\int_{0}^{t} \int_{0}^{T} x\left(\tau_{1}\right) d \tau, d \tau \\
x(t)=e^{t A} x(0)+\int_{0}^{T} e^{\tau A} d \tau b & \dot{x}=A x+b
\end{array}
$$

We compute the first two terms as:

$$
\begin{array}{lll}
x_{\text {ln }} t(t)=e^{t A_{1}}\left[\begin{array}{c}
O_{n+1} \\
1
\end{array}\right] & A_{1} \triangleq\left[\begin{array}{cc}
A_{0} & x_{0}(0) \\
0 & 0
\end{array}\right] & A_{0}=\left[\begin{array}{cc}
A & b \\
0 & 0
\end{array}\right] \\
x_{\text {int }}(t)=e^{\dagger A_{2}}\left[\begin{array}{c}
0_{n+2} \\
1
\end{array}\right] & A_{2} \triangleq\left[\begin{array}{ccc}
A_{0} & x_{0}(0) & 0 \\
0 & 0 & 1 \\
0 & 0 & 0
\end{array}\right] & x_{0}(0)=\left[\begin{array}{c}
x(0) \\
1
\end{array}\right]
\end{array}
$$

Actually computations could be faster by having zero initial conditions

$$
\begin{aligned}
& \dot{x}(t)=A x(t)+b \quad \bar{x}(t) \triangleq x(t)-x(0) \Rightarrow \bar{x}(0)=0 \\
& \dot{\bar{x}}(t)=\dot{x}(t)=A(x(t)-x(0))+b=A x(t)+\underbrace{b-A x(0)}_{\bar{b}} \\
& \bar{x}(t)=\int_{0}^{t} e^{\tau A} d \tau \bar{b} \Rightarrow x(t)=x(0)+\bar{x}(t)=x(0)+\int_{0}^{t} e^{\tau A} d \tau(b-A x(0))
\end{aligned}
$$

Using this expression I can move $x(0)$ inside $\bar{b}$ so $A_{1}, A_{2}$ become

$$
\begin{aligned}
& A_{1} \triangleq\left[\begin{array}{c|c|c}
A & b & 0 \\
\hline 0 & 0 & 1 \\
\hline 0 & 0 & 0
\end{array}\right] \\
& A_{2} \triangleq\left[\begin{array}{c|c|cc}
A & b & 0 & 0 \\
\hline 0 & 0 & 1 & 0 \\
\hline 0 & 0 & 0 & 1 \\
0 & 0 & 0 & 0
\end{array}\right]
\end{aligned}
$$

So to compute expo of $A_{1}$ and $A_{2}$ we need powers of $A_{1}, A_{2}$ :

$$
\begin{aligned}
& A_{1}^{2}=\left[\begin{array}{lll}
A & \bar{b} & 0 \\
0 & 0 & 1 \\
0 & 0 & 0
\end{array}\right]\left[\begin{array}{lll}
A & \bar{b} & 0 \\
0 & 0 & 1 \\
0 & 0 & 0
\end{array}\right]=\left[\begin{array}{ccc}
A^{2} & A \bar{b} & \bar{b} \\
0 & 0 & 0 \\
0 & 0 & 0
\end{array}\right] \\
& A_{1}^{3}=\left[\begin{array}{ccc}
A^{2} & A \bar{b} & \bar{b} \\
0 & 0 & 0 \\
0 & 0 & 0
\end{array}\right]\left[\begin{array}{ccc}
A & \bar{b} & 0 \\
0 & 0 & 1 \\
0 & 0 & 0
\end{array}\right]=\left[\begin{array}{ccc}
A^{3} & A^{2} \bar{b} & A \bar{b} \\
0 & 0 & 0 \\
0 & 0 & 0
\end{array}\right]
\end{aligned}
$$

$$
A_{1}^{k}=\left[\begin{array}{ccc}
A^{k} & A^{k-1} b & A^{k-2} b \\
0 & 0 & 0 \\
0 & 0 & 0
\end{array}\right] \quad \Delta=W_{e} \text { only need powers of } A \text { ! }
$$

$$
A_{2}^{2}=\left[\begin{array}{llll}
A & - & 0 & 0 \\
0 & 0 & 1 & 0 \\
0 & 0 & 0 & 1 \\
0 & 0 & 0 & 0
\end{array}\right]\left[\begin{array}{cccc}
A & -b & 0 & 0 \\
0 & 0 & 1 & 0 \\
0 & 0 & 0 & 1 \\
0 & 0 & 0 & 0
\end{array}\right]=\left[\begin{array}{cccc}
A^{2} & A \bar{b} & b & 0 \\
0 & 0 & 0 & 0 \\
0 & 0 & 0 & 0 \\
0 & 0 & 0 & 0
\end{array}\right]=\left[\begin{array}{cc}
A_{1}^{2} & 0 \\
0 & 0
\end{array}\right]
$$

$$
A_{2}^{3}=\left[\begin{array}{cccc}
A^{2} & A \bar{b} & \bar{b} & 0 \\
0 & 0 & 0 & 0 \\
0 & 0 & 0 & 0 \\
0 & 0 & 0 & 0
\end{array}\right]\left[\begin{array}{cccc}
A & \bar{b} & 0 & 0 \\
0 & 0 & 1 & 0 \\
0 & 0 & 0 & 1 \\
0 & 0 & 0 & 0
\end{array}\right]=\left[\begin{array}{cccc}
A^{3} & A^{2} b & A \bar{b} & b \\
0 & 0 & 0 & 0 \\
0 & 0 & 0 & 0 \\
0 & 0 & 0 & 0
\end{array}\right]=\left[\begin{array}{cc}
A_{1}^{3} & \bar{b} \\
0 \\
0 & 0
\end{array}\right]
$$

$$
A_{2}^{4}=\left[\begin{array}{cccc}
A^{3} & A^{2} \bar{b} & A \bar{b} & \bar{b} \\
0 & 0 & 0 & 0 \\
0 & 0 & 0 & 0 \\
0 & 0 & 0 & 0
\end{array}\right]\left[\begin{array}{cccc}
A & \bar{b} & 0 & 0 \\
0 & 0 & 1 & 0 \\
0 & 0 & 0 & 1 \\
0 & 0 & 0 & 0
\end{array}\right]=\left[\begin{array}{cccc}
A^{3} & A^{3} \bar{b} & A^{2} \bar{b} & A \bar{b} \\
0 & 0 & 0 & 0 \\
0 & 0 & 0 & 0 \\
0 & 0 & 0 & 0
\end{array}\right]
$$

$A_{2}^{k}=\left[\begin{array}{cccc}A^{k} & A^{k-1} \bar{b} & A^{k-2} \bar{b} & A^{k-3} \dot{b} \\ 0 & 0 & 0 & 0 \\ 0 & 0 & 0 & 0 \\ 0 & 0 & 0 & 0\end{array}\right]\{=$ We only need powers of $A$

Basically, once we have computed powers of $A$, then computing powers of $A_{1}$ and $A_{2}$ is very cheop! The only remaining operation in expm is the inverse of a polynomial of $A_{1} / A_{2}$. I am hopeful that even these two inverses could be easily computed together saving computation time. The derivation of their expressions should follow the some approach used above for deriving the inverse of $M$.

